util.dfy
@@ -75,24 +75,11 @@ lemma notempty<K,V>(s: set<K>, m: map<K,V>)
     ensures |s| >= 1 ==> |m| >= 1
 {}
 
-function map_not_empty<A,B>(xs: set<A>, m: map<A,B>):  (ys: set<B>)
+function map_not_empty<A(!new),B>(xs: set<A>, m: map<A,B>):  (ys: set<B>)
     requires xs == m.Keys
     ensures ys == m.Values
     ensures |xs| >= 1 ==> |ys| >= 1
-    ensures forall x :: x in xs ==> m[x] in ys
+    ensures forall x :: true ==> (x in xs <==> x in m.Keys && m[x] in ys)
 {
     m.Values
-}
-
-function map_set<A(!new),B>(xs: set<A>, f: (A) -> B) :  (ys: set<B>)
-    requires forall x {:trigger f.requires(x)}{:trigger x in xs} :: x in xs ==> f.requires(x)
-    ensures |xs| >= 1 ==> |ys| >= 1
-    ensures ys == (set i | i in xs :: f(i))
-    ensures forall i :: i in xs ==> f(i) in ys
-{
-    var ys := set i | i in xs :: f(i);
-    ghost var ys_map := map i | i in xs :: f(i);
-    assert xs == ys_map.Keys;
-    assert ys == ys_map.Values;
-    ys
 }
